disk-betree/BetreeAsyncBlockCacheSystem_Refines_ThreeStateVersionedPivotBetree.dfy
@@ -1,0 +1,165 @@
+include "AsyncDiskModel.dfy"
+include "PivotBetree_Refines_Betree.dfy"
+include "AsyncBlockCache.dfy"
+include "../lib/Maps.dfy"
+include "../lib/sequences.dfy"
+include "AsyncBlockCacheSystem.dfy"
+include "BetreeAsyncBlockCache.dfy"
+include "AsyncBlockCacheSystem_Refines_ThreeStateVersionedBlockInterface.dfy"
+include "ThreeStateVersionedPivotBetree.dfy"
+include "BetreeAsyncBlockCacheSystem.dfy"
+
+module BetreeAsyncBlockCacheSystem_Refines_ThreeStateVersionedPivotBetree {
+  import opened Maps
+  import opened Sequences
+
+  import BBCS = BetreeAsyncBlockCacheSystem
+  import TSV = ThreeStateVersionedPivotBetree
+
+  import opened PivotBetreeSpec`Spec
+  import BC = BetreeGraphAsyncBlockCache
+  import BCS = BetreeGraphAsyncBlockCacheSystem
+  import BT = PivotBetree
+  import BTI = PivotBetreeInvAndRefinement
+  import BI = PivotBetreeBlockInterface
+  import Ref = AsyncBlockCacheSystem_Refines_ThreeStateVersionedBlockInterface
+  import D = AsyncDisk
+
+  import M = BetreeAsyncBlockCache
+  type UIOp = BBCS.UIOp
+
+  function Ik(k: BBCS.Constants) : TSV.Constants
+  {
+    TSV.Constants(BT.Constants(BI.Constants()))
+  }
+
+  function I(k: BBCS.Constants, s: BBCS.Variables) : TSV.Variables
+  requires BBCS.Inv(k, s)
+  {
+    TSV.Variables(
+      BBCS.PersistentBetree(k, s),
+      BBCS.FrozenBetree(k, s),
+      BBCS.EphemeralBetree(k, s),
+      map[] // TODO
+    )
+  }
+
+  // Proofs
+
+  lemma RefinesInit(k: BBCS.Constants, s: BBCS.Variables)
+    requires BBCS.Init(k, s)
+    ensures BBCS.Inv(k, s)
+    ensures TSV.Init(Ik(k), I(k, s))
+  {
+    BCS.InitImpliesInv(k, s);
+    BTI.InitImpliesInv(Ik(k).k, BBCS.PersistentBetree(k, s));
+    Ref.InitImpliesGraphsEq(k, s);
+  }
+
+  lemma BetreeMoveStepRefines(k: BBCS.Constants, s: BBCS.Variables, s': BBCS.Variables, uiop: UIOp, dop: M.DiskOp, betreeStep: BetreeStep)
+    requires BBCS.Inv(k, s)
+    requires M.BetreeMove(k.machine, s.machine, s'.machine, uiop, dop, betreeStep)
+    requires D.Next(k.disk, s.disk, s'.disk, dop)
+    ensures BBCS.Inv(k, s')
+    ensures TSV.Next(Ik(k), I(k, s), I(k, s'), uiop)
+  {
+    Ref.StepGraphs(k, s, s', BCS.MachineStep(dop, BC.TransactionStep(BetreeStepOps(betreeStep))));
+    Ref.RefinesReads(k, s, BetreeStepReads(betreeStep));
+    assert BT.NextStep(Ik(k).k, BBCS.EphemeralBetree(k, s), BBCS.EphemeralBetree(k, s'), uiop, BT.BetreeStep(betreeStep));
+    BTI.NextPreservesInv(Ik(k).k, BBCS.EphemeralBetree(k, s), BBCS.EphemeralBetree(k, s'), uiop);
+
+    assert TSV.Move3(Ik(k), I(k, s), I(k, s'), uiop);
+    assert TSV.NextStep(Ik(k), I(k, s), I(k, s'), uiop, TSV.Move3Step);
+  }
+
+  lemma BlockCacheMoveStepRefines(k: BBCS.Constants, s: BBCS.Variables, s': BBCS.Variables, uiop: UIOp, dop: M.DiskOp, step: BC.Step)
+    requires BBCS.Inv(k, s)
+    requires !step.TransactionStep?
+    requires M.BlockCacheMove(k.machine, s.machine, s'.machine, uiop, dop, step)
+    requires uiop.NoOp?
+    requires D.Next(k.disk, s.disk, s'.disk, dop)
+    ensures BBCS.Inv(k, s')
+    ensures TSV.Next(Ik(k), I(k, s), I(k, s'), uiop)
+  {
+    Ref.StepGraphs(k, s, s', BCS.MachineStep(dop, step));
+    if (step.UnallocStep?) {
+      //assert BI.GC(Ik(k).bck, EphemeralBetree(k, s).bcv, s'.bcv, refs)
+      Ref.UnallocStepMeetsGCConditions(k, s, s', dop, step.ref);
+      /*assert step.ref in EphemeralBetree(k, s).bcv.view;
+      assert iset{step.ref} !! BI.LiveReferences(Ik(k).bck, EphemeralBetree(k, s).bcv);
+      assert BI.ClosedUnderPredecessor(EphemeralBetree(k, s).bcv.view, iset{step.ref});
+      assert IMapRemove1(EphemeralBetree(k, s).bcv.view, step.ref)
+          == IMapRemove(EphemeralBetree(k, s).bcv.view, iset{step.ref});*/
+      assert BT.GC(Ik(k).k, BBCS.EphemeralBetree(k, s), BBCS.EphemeralBetree(k, s'), uiop, iset{step.ref});
+      BTI.GCStepRefines(Ik(k).k, BBCS.EphemeralBetree(k, s), BBCS.EphemeralBetree(k, s'), uiop, iset{step.ref});
+
+      assert BT.NextStep(Ik(k).k, I(k, s).s3, I(k, s').s3, uiop, BT.GCStep(iset{step.ref}));
+      assert TSV.NextStep(Ik(k), I(k, s), I(k, s'), uiop, TSV.Move3Step);
+    } else {
+      if (TSV.NextStep(Ik(k), I(k, s), I(k, s'), uiop, TSV.Move2to3Step)) {
+        // freeze case
+        assert TSV.Next(Ik(k), I(k, s), I(k, s'), uiop);
+      } else {
+        // everything else is a no-op
+        assert BT.NextStep(Ik(k).k, I(k, s).s3, I(k, s').s3, uiop, BT.StutterStep);
+        assert TSV.NextStep(Ik(k), I(k, s), I(k, s'), uiop, TSV.Move3Step);
+      }
+    }
+  }
+
+  lemma CrashStepRefines(k: BBCS.Constants, s: BBCS.Variables, s': BBCS.Variables, uiop: UIOp)
+    requires BBCS.Inv(k, s)
+    requires BBCS.Crash(k, s, s', uiop)
+    ensures BBCS.Inv(k, s')
+    ensures TSV.Next(Ik(k), I(k, s), I(k, s'), uiop)
+  {
+    Ref.StepGraphs(k, s, s', BCS.CrashStep);
+    assert TSV.NextStep(Ik(k), I(k, s), I(k, s'), uiop, TSV.CrashStep);
+  }
+
+  lemma DiskInternalStepRefines(k: BBCS.Constants, s: BBCS.Variables, s': BBCS.Variables, uiop: UIOp, step: D.InternalStep)
+    requires BBCS.Inv(k, s)
+    requires BBCS.DiskInternal(k, s, s', uiop, step)
+    requires uiop.NoOp?
+    ensures BBCS.Inv(k, s')
+    ensures TSV.Next(Ik(k), I(k, s), I(k, s'), uiop)
+  {
+    Ref.StepGraphs(k, s, s', BCS.DiskInternalStep(step));
+    if (TSV.NextStep(Ik(k), I(k, s), I(k, s'), uiop, TSV.Move1to2Step)) {
+      assert TSV.Next(Ik(k), I(k, s), I(k, s'), uiop);
+    } else {
+      assert BT.NextStep(Ik(k).k, I(k, s).s3, I(k, s').s3, uiop, BT.StutterStep);
+      assert TSV.Move3(Ik(k), I(k, s), I(k, s'), uiop);
+      assert TSV.NextStep(Ik(k), I(k, s), I(k, s'), uiop, TSV.Move3Step);
+    }
+  }
+
+  lemma NextStepRefines(k: BBCS.Constants, s: BBCS.Variables, s': BBCS.Variables, uiop: UIOp, step: BBCS.Step)
+    requires BBCS.Inv(k, s)
+    requires BBCS.NextStep(k, s, s', uiop, step)
+    ensures BBCS.Inv(k, s')
+    ensures TSV.Next(Ik(k), I(k, s), I(k, s'), uiop)
+  {
+    match step {
+      case MachineStep(dop) => {
+        var machineStep :| M.NextStep(k.machine, s.machine, s'.machine, uiop, dop, machineStep);
+        match machineStep {
+          case BetreeMoveStep(betreeStep) => BetreeMoveStepRefines(k, s, s', uiop, dop, betreeStep);
+          case BlockCacheMoveStep(blockCacheStep) => BlockCacheMoveStepRefines(k, s, s', uiop, dop, blockCacheStep);
+        }
+      }
+      case DiskInternalStep(step) => DiskInternalStepRefines(k, s, s', uiop, step);
+      case CrashStep => CrashStepRefines(k, s, s', uiop);
+    }
+  }
+
+  lemma RefinesNext(k: BBCS.Constants, s: BBCS.Variables, s': BBCS.Variables, uiop: UIOp)
+    requires BBCS.Inv(k, s)
+    requires BBCS.Next(k, s, s', uiop)
+    ensures BBCS.Inv(k, s')
+    ensures TSV.Next(Ik(k), I(k, s), I(k, s'), uiop);
+  {
+    var step :| BBCS.NextStep(k, s, s', uiop, step);
+    NextStepRefines(k, s, s', uiop, step);
+  }
+}
