disk-betree/ThreeStateVersionedPivotBetree.dfy
@@ -1,6 +1,6 @@
 include "ThreeStateVersioned.dfy"
 include "PivotBetree.dfy"
 
-module ThreeStateVersionedPivotBetree {
+module ThreeStateVersionedPivotBetree refines ThreeStateVersioned {
   import SM = PivotBetree
 }
